do not use tuples in Semantics, Memory

bedrock2/src/bedrock2/Memory.v
@@ -1,5 +1,6 @@
-Require Import Coq.ZArith.ZArith.
-Require Import coqutil.Z.Lia.
+Require Export coqutil.Map.OfListWord coqutil.Map.Memory.
+
+From Coq Require Import ZArith Lia.
 Require Coq.Lists.List.
 Require Import coqutil.sanity.
 Require Import coqutil.Decidable.
@@ -9,197 +10,104 @@ Require Import coqutil.Tactics.Tactics coqutil.Datatypes.Option.
 Require Import BinIntDef coqutil.Word.Interface coqutil.Word.LittleEndianList.
 Require Import bedrock2.Syntax.
 Require Import coqutil.Byte.
-Require Import coqutil.Map.OfListWord.
 
 Open Scope Z_scope.
 
-Definition bytes_per_word(width: Z): Z := (width + 7) / 8.
+Definition bytes_per_word width : Z := (width + 7) / 8.
 
-Module WithoutTuples. Section Memory.
+Definition bytes_per {width} sz :=
+  match sz with
+    | access_size.one => 1 | access_size.two => 2 | access_size.four => 4
+    | access_size.word => Z.to_nat (bytes_per_word width)
+  end%nat.
+
+Definition load {width} {word : word width} {mem : map.map word byte}
+  sz (m : mem) (a: word): option word :=
+  match load_Z m a (bytes_per (width:=width) sz) with
+  | Some z => Some (word.of_Z z)
+  | None => None
+  end.
+
+Definition store {width} {word : word width} {mem : map.map word byte}
+  sz (m : mem) (a v : word) : option mem :=
+  store_Z m a (bytes_per (width:=width) sz) (word.unsigned v).
+
+Definition anybytes {width} {word : word width} {mem : map.map word byte}
+  (a : word) (n : Z) (m : mem) :=
+  exists bs: list byte, map.of_list_word_at a bs = m /\
+  Z.of_nat (length bs) = n /\ Z.of_nat (length bs) <= 2 ^ width.
+
+Lemma anybytes_unique_domain {width} {word : word width} {mem : map.map word byte}
+  {mem_ok: map.ok mem} {word_ok: word.ok word} a n (m1 m2 : mem) :
+  anybytes a n m1 -> anybytes a n m2 -> map.same_domain m1 m2.
+Proof.
+  cbv [anybytes]; intros (?&?&?) (?&?&?); subst.
+  cbv [map.same_domain map.sub_domain].
+  setoid_rewrite @map.get_of_list_word_at; try exact _; split; intros *.
+  2: destruct List.nth_error eqn:A, (List.nth_error x) eqn:B.
+  1: destruct List.nth_error eqn:A, (List.nth_error x0) eqn:B.
+  all: intros; try congruence; eauto.
+  all: rewrite List.nth_error_None in B.
+  all: epose proof proj1 ((List.nth_error_Some _ _)) as HH; rewrite A in HH.
+  all : specialize (HH ltac:(discriminate)); lia.
+Qed.
+
+Section Deprecated. (* The below functions needlessly use tuples for what can be done with lists *)
   Context {width: Z} {word: word width} {mem: map.map word byte}.
-  Definition footprint (a : word) (n : nat) : list word :=
-    List.map (fun i => word.add a (word.of_Z (Z.of_nat i))) (List.seq 0 n).
-  Definition load_bytes (m : mem) (a : word) (n : nat) : option (list byte) :=
-    option_all (List.map (map.get m) (footprint a n)).
-  Definition unchecked_store_bytes (m : mem) (a : word) (bs : list byte) :=
-    map.putmany m (map.of_list_word_at a bs).
-  Definition store_bytes (m : mem)(a : word) (bs : list byte): option mem :=
-    match load_bytes m a (length bs) with
-    | Some _ => Some (unchecked_store_bytes m a bs)
-    | None => None (* some addresses were invalid *)
-    end.
-
-  Local Notation "a [ i ]" := (List.nth_error a i) (at level 9, format "a [ i ]").
-
-  Lemma length_footprint a n : length (footprint a n) = n.
-  Proof. cbv [footprint]. rewrite List.map_length, List.seq_length; trivial. Qed.
-  Lemma nth_error_footprint_inbounds a n i (H : lt i n)
-    : (footprint a n)[i] = Some (word.add a (word.of_Z (Z.of_nat i))).
-  Proof.
-    cbv [footprint].
-    erewrite List.map_nth_error; trivial.
-    rewrite List.nth_error_nth' with (d:=O); rewrite ?List.seq_length; trivial; [].
-    rewrite List.seq_nth; trivial.
-  Qed.
-
-  Lemma length_load_bytes m a n bs (H : load_bytes m a n = Some bs)
-    : length bs = n.
-  Proof.
-    eapply length_option_all in H.
-    pose proof length_footprint a n.
-    pose proof List.map_length (map.get m) (footprint a n).
-    congruence.
-  Qed.
-  Lemma nth_error_load_bytes m a n bs (H : load_bytes m a n = Some bs) i (Hi : lt i n)
-    : List.nth_error bs i = map.get m (word.add a (word.of_Z (Z.of_nat i))).
-  Proof.
-    cbv [load_bytes] in *.
-    epose proof @nth_error_option_all _ _ _ _ H as Hii.
-    rewrite List.map_length, length_footprint in Hii.
-    case (Hii Hi) as (b&Hbl&Hbr); clear Hii; rewrite Hbr; clear Hbr.
-    erewrite List.map_nth_error in Hbl by eauto using nth_error_footprint_inbounds.
-    injection Hbl; congruence.
-  Qed.
-
-  Lemma load_bytes_None m a n (H : load_bytes m a n = None)
-    : exists i, lt i n /\ map.get m (word.add a (word.of_Z (Z.of_nat i))) = None.
-  Proof.
-    eapply option_all_None in H; case H as (i&Hi); exists i.
-    eapply nth_error_map_Some in Hi; case Hi as (x&Hfx&Hmx).
-    pose proof proj1 (List.nth_error_Some (footprint a n) i) ltac:(congruence).
-    rewrite length_footprint in H; split; trivial.
-    eapply nth_error_footprint_inbounds with (a:=a) in H.
-    congruence.
-  Qed.
-
-  Lemma load_bytes_all m a n
-    (H : forall i, lt i n -> exists b, map.get m (word.add a (word.of_Z (Z.of_nat i))) = Some b)
-    : exists bs, load_bytes m a n = Some bs.
-  Proof.
-    destruct (load_bytes m a n) eqn:HX; eauto.
-    eapply load_bytes_None in HX; destruct HX as (?&?&?). firstorder congruence.
-    exact nil.
-  Qed.
-
-  Import Word.Properties.
-  Context {mem_ok: map.ok mem} {word_ok: word.ok word}.
-  Local Infix "$+" := map.putmany (at level 70).
-  Local Notation "xs $@ a" := (map.of_list_word_at a xs) (at level 10, format "xs $@ a").
-  Lemma load_bytes_of_putmany_bytes_at bs a mR n (Hn : length bs = n) (Hl : Z.of_nat n < 2^width)
-    : load_bytes (mR $+ bs$@a) a n = Some bs.
-  Proof.
-    destruct (load_bytes (mR $+ bs$@a) a n) eqn:HN in *; cycle 1.
-    { exfalso; eapply load_bytes_None in HN; case HN as (i&?&?).
-      case (Properties.map.putmany_spec mR (bs$@a) (word.add a (word.of_Z (BinIntDef.Z.of_nat i)))) as [(?&?&?)| (?&?) ]; try congruence.
-      rewrite map.get_of_list_word_at in H1; eapply List.nth_error_None in H1.
-      revert H1.
-      rewrite word.word_sub_add_l_same_l, word.unsigned_of_Z.
-      cbv [word.wrap]; rewrite Z.mod_small, Znat.Nat2Z.id; eauto; blia. }
-    transitivity (Some l); try congruence; f_equal; subst n.
-    symmetry; eapply List.nth_error_ext_samelength.
-    { symmetry; eauto using length_load_bytes. }
-    intros.
-    pose proof nth_error_load_bytes _ a _ _ HN i ltac:(trivial) as HH.
-    epose proof H; eapply List.nth_error_nth' with (d:=Byte.x00) in H.
-    erewrite Properties.map.get_putmany_right in HH; cycle 1.
-    { rewrite map.get_of_list_word_at.
-      rewrite word.word_sub_add_l_same_l, word.unsigned_of_Z.
-      cbv [word.wrap]; rewrite Z.mod_small, Znat.Nat2Z.id; eauto; blia. }
-    congruence.
-  Qed.
-End Memory. End WithoutTuples.
-
-Section Memory.
-  Context {width: Z} {word: word width} {mem: map.map word byte}.
-
-  Definition ftprint(a: word)(n: Z): list word :=
-    List.unfoldn (fun w => word.add w (word.of_Z 1)) (Z.to_nat n) a.
-
-  Definition anybytes(a: word)(n: Z)(m: mem): Prop :=
-    exists bytes: list byte, map.of_disjoint_list_zip (ftprint a n) bytes = Some m.
-
+  (* deprecated since 2025 *)
   Definition footprint(a: word)(sz: nat): tuple word sz :=
     tuple.unfoldn (fun w => word.add w (word.of_Z 1)) sz a.
 
+  (* deprecated since 2025 *)
   Definition load_bytes(sz: nat)(m: mem)(addr: word): option (tuple byte sz) :=
     map.getmany_of_tuple m (footprint addr sz).
 
+  (* deprecated since 2025 *)
   Definition unchecked_store_bytes(sz: nat)(m: mem)(a: word)(bs: tuple byte sz): mem :=
     map.putmany_of_tuple (footprint a sz) bs m.
 
+  (* deprecated since 2025 *)
   Definition store_bytes(sz: nat)(m: mem)(a: word)(v: tuple byte sz): option mem :=
     match load_bytes sz m a with
     | Some _ => Some (unchecked_store_bytes sz m a v)
     | None => None (* some addresses were invalid *)
     end.
 
-  Definition bytes_per sz :=
-    match sz with
-      | access_size.one => 1 | access_size.two => 2 | access_size.four => 4
-      | access_size.word => Z.to_nat (bytes_per_word width)
-    end%nat.
-
-  Definition load_Z(sz: access_size)(m: mem)(a: word): option Z :=
-    match load_bytes (bytes_per sz) m a with
-    | Some bs => Some (LittleEndianList.le_combine (tuple.to_list bs))
-    | None => None
-    end.
-
-  Definition store_Z(sz: access_size)(m: mem)(a: word)(v: Z): option mem :=
-    store_bytes _ m a (tuple.of_list (LittleEndianList.le_split (bytes_per sz) v)).
-
-  Definition load(sz: access_size)(m: mem)(a: word): option word :=
-    match load_Z sz m a with
-    | Some v => Some (word.of_Z v)
-    | None => None
-    end.
-
-  Definition store(sz: access_size)(m: mem)(a: word)(v: word): option mem :=
-    store_Z sz m a (word.unsigned v).
-
-  Lemma load_None: forall sz m a,
-      8 <= width -> (* note: [0 < width] is sufficient *)
-      map.get m a = None ->
-      load sz m a = None.
-  Proof.
-    intros. destruct sz; cbv [load load_Z load_bytes map.getmany_of_tuple footprint bytes_per bytes_per_word tuple.option_all tuple.map tuple.unfoldn];
-    try solve [ rewrite H0; reflexivity].
-    destruct (Z.to_nat ((width + 7) / 8)) eqn: E.
-    - exfalso.
-      assert (0 < (width + 7) / 8) as A. {
-        apply Z.div_str_pos. blia.
-      }
-      change O with (Z.to_nat 0) in E.
-      apply Z2Nat.inj in E; blia.
-    - cbv [tuple.option_all tuple.map tuple.unfoldn].
-      rewrite H0.
-      reflexivity.
-  Qed.
-
   Context {mem_ok: map.ok mem}.
   Context {word_ok: word.ok word}.
 
-  Lemma store_preserves_domain: forall sz m a v m',
-      store sz m a v = Some m' -> map.same_domain m m'.
+  Lemma to_list_footprint a sz :
+    tuple.to_list (footprint a sz) = coqutil.Map.Memory.footprint a sz.
   Proof.
-    destruct sz;
-      cbv [store store_Z store_bytes bytes_per load_bytes unchecked_store_bytes];
-      intros;
-      (destruct_one_match_hyp; [|discriminate]);
-      inversion_option;
-      subst;
-      eapply map.putmany_of_tuple_preserves_domain;
-      eassumption.
+    revert a; induction sz; cbn; intros; f_equal.
+    { rewrite Properties.word.add_0_r; trivial. }
+    { cbv [footprint] in IHsz. rewrite IHsz, <-List.seq_shift, List.map_map.
+      eapply List.map_ext; intros.
+      rewrite Nat2Z.inj_succ; cbv [BinInt.Z.succ]; rewrite Properties.word.ring_morph_add.
+      rewrite <-!Properties.word.add_assoc; f_equal.
+      rewrite Properties.word.add_comm; f_equal. }
   Qed.
 
-  Lemma anybytes_unique_domain: forall a n m1 m2,
-      anybytes a n m1 ->
-      anybytes a n m2 ->
-      map.same_domain m1 m2.
+  Lemma to_list_load_bytes sz m a :
+    option_map tuple.to_list (load_bytes sz m a) = coqutil.Map.Memory.load_bytes m a sz.
   Proof.
-    unfold anybytes. intros.
-    destruct H as [vs1 ?]. destruct H0 as [vs2 ?].
-    eapply map.of_disjoint_list_zip_same_domain; eassumption.
+    cbv [load_bytes]. rewrite map.to_list_getmany_of_tuple, to_list_footprint; trivial.
   Qed.
 
-End Memory.
+  Lemma unchecked_store_bytes_correct sz m a bs :
+    unchecked_store_bytes sz m a bs = coqutil.Map.Memory.unchecked_store_bytes m a (tuple.to_list bs).
+  Proof.
+    cbv [unchecked_store_bytes coqutil.Map.Memory.unchecked_store_bytes].
+    revert a; induction sz; cbn; intros; rewrite ?map.of_list_word_nil, ?map.putmany_empty_r; trivial.
+    rewrite map.of_list_word_at_cons, <-map.put_putmany_commute; f_equal.
+    erewrite <-IHsz; trivial.
+  Qed.
+
+  Lemma store_bytes_correct sz m a bs :
+    store_bytes sz m a bs = coqutil.Map.Memory.store_bytes m a (tuple.to_list bs).
+  Proof.
+    cbv [store_bytes coqutil.Map.Memory.store_bytes].
+    rewrite <-to_list_load_bytes, tuple.length_to_list; case load_bytes as []; cbn; trivial.
+    rewrite unchecked_store_bytes_correct; trivial.
+  Qed.
+End Deprecated.
